left lemma working

reduction_directedHamiltonianCircuit_to_hamiltonianCircuit/left_lemma_working_file.dfy
@@ -46,148 +46,148 @@ module LeftLemma
         ensures forall i :: 0<=i<|c| ==> isUndirectedHamiltonianCircuit(g, cicle_sequence(c, i))
     {}
 
-    ghost predicate in_out_circuit(g: Graph, c: seq<nat>)
-        requires validUndirectedGraph(g)
-        requires |g|>2 && |g|%3==0
-        requires in_out_graph(g)
-        // requires isUndirectedHamiltonianCircuit(g, uc)
-    {
-        isUndirectedHamiltonianCircuit(g, c)
-        &&
-        (
-            (forall i :: 0<i<|c|-1 ==> way1(g, c, i))
-            ||
-            (forall i :: 0<i<|c|-1 ==> way2(g, c, i))
-        )
-    }
+    // ghost predicate in_out_circuit(g: Graph, c: seq<nat>)
+    //     requires validUndirectedGraph(g)
+    //     requires |g|>2 && |g|%3==0
+    //     requires in_out_graph(g)
+    //     // requires isUndirectedHamiltonianCircuit(g, uc)
+    // {
+    //     isUndirectedHamiltonianCircuit(g, c)
+    //     &&
+    //     (
+    //         (forall i :: 0<i<|c|-1 ==> way1(g, c, i))
+    //         ||
+    //         (forall i :: 0<i<|c|-1 ==> way2(g, c, i))
+    //     )
+    // }
 
-    //circuit has structure in->og->out
-    ghost predicate way1(g: Graph, c: seq<nat>, i: int)
-        requires validUndirectedGraph(g)
-        requires |g|>2 && |g|%3==0
-        requires in_out_graph(g)
-        requires 0<i<|c|-1
-    {
-        (0<=c[i]<|g|/3 ==>  //case og node
-        (
-            c[i-1]==c[i]+(|g|/3)*2  //before: in
-            &&
-            c[i+1]==c[i]+|g|/3    //next: out
-        ))
-        &&
-        (|g|/3<=c[i]<(|g|/3)*2 ==>  //case out node
-        (
-            c[i-1]==c[i]-|g|/3   //before: og
-            &&
-            (|g|/3)*2<=c[i+1]<|g|   //next: in (range)
-        ))
-        &&
-        ((|g|/3)*2<=c[i]<|g| ==>  //case in node
-        (
-            |g|/3<=c[i-1]<(|g|/3)*2   //before: out (range)
-            &&
-            c[i+1]==c[i]-(|g|/3)*2    //next: og
-        ))
-    }
+    // //circuit has structure in->og->out
+    // ghost predicate way1(g: Graph, c: seq<nat>, i: int)
+    //     requires validUndirectedGraph(g)
+    //     requires |g|>2 && |g|%3==0
+    //     requires in_out_graph(g)
+    //     requires 0<i<|c|-1
+    // {
+    //     (0<=c[i]<|g|/3 ==>  //case og node
+    //     (
+    //         c[i-1]==c[i]+(|g|/3)*2  //before: in
+    //         &&
+    //         c[i+1]==c[i]+|g|/3    //next: out
+    //     ))
+    //     &&
+    //     (|g|/3<=c[i]<(|g|/3)*2 ==>  //case out node
+    //     (
+    //         c[i-1]==c[i]-|g|/3   //before: og
+    //         &&
+    //         (|g|/3)*2<=c[i+1]<|g|   //next: in (range)
+    //     ))
+    //     &&
+    //     ((|g|/3)*2<=c[i]<|g| ==>  //case in node
+    //     (
+    //         |g|/3<=c[i-1]<(|g|/3)*2   //before: out (range)
+    //         &&
+    //         c[i+1]==c[i]-(|g|/3)*2    //next: og
+    //     ))
+    // }
 
-    //circuit has structure out->og->in
-    ghost predicate way2(g: Graph, c: seq<nat>, i: int)
-    requires validUndirectedGraph(g)
-    requires |g|>2 && |g|%3==0
-    requires in_out_graph(g)
-    requires 0<i<|c|-1
-    {
-        (0<=c[i]<|g|/3 ==>  //case og node
-        (
-            c[i-1]==c[i]+|g|/3    //before: out
-            &&
-            c[i+1]==c[i]+(|g|/3)*2  //next: in
-        ))
-        &&
-        (|g|/3<=c[i]<(|g|/3)*2 ==>  //case out node
-        (
-            (|g|/3)*2<=c[i-1]<|g|   //before: in (range)
-            &&
-            c[i+1]==c[i]-|g|/3   //next: og
-        ))
-        &&
-        ((|g|/3)*2<=c[i]<|g| ==>  //case in node
-        (
-            c[i-1]==c[i]-(|g|/3)*2    //before: og
-            &&
-            |g|/3<=c[i+1]<(|g|/3)*2   //next: out (range)
-        ))
-    }
+    // //circuit has structure out->og->in
+    // ghost predicate way2(g: Graph, c: seq<nat>, i: int)
+    // requires validUndirectedGraph(g)
+    // requires |g|>2 && |g|%3==0
+    // requires in_out_graph(g)
+    // requires 0<i<|c|-1
+    // {
+    //     (0<=c[i]<|g|/3 ==>  //case og node
+    //     (
+    //         c[i-1]==c[i]+|g|/3    //before: out
+    //         &&
+    //         c[i+1]==c[i]+(|g|/3)*2  //next: in
+    //     ))
+    //     &&
+    //     (|g|/3<=c[i]<(|g|/3)*2 ==>  //case out node
+    //     (
+    //         (|g|/3)*2<=c[i-1]<|g|   //before: in (range)
+    //         &&
+    //         c[i+1]==c[i]-|g|/3   //next: og
+    //     ))
+    //     &&
+    //     ((|g|/3)*2<=c[i]<|g| ==>  //case in node
+    //     (
+    //         c[i-1]==c[i]-(|g|/3)*2    //before: og
+    //         &&
+    //         |g|/3<=c[i+1]<(|g|/3)*2   //next: out (range)
+    //     ))
+    // }
 
-    lemma in_out_circuit_lemma(g: Graph, c: seq<nat>)
-        requires validUndirectedGraph(g)
-        requires |g|>2 && |g|%3==0
-        requires isUndirectedHamiltonianCircuit(g, c)
-        requires in_out_graph(g)
-        ensures in_out_circuit(g, c)
-    {
-        assert (forall i :: 0<i<|c|-1 ==> way2(g, c, i)) ==> (forall i :: 0<i<|c|-1 ==> way1(g, rSeq(c), i));
-        forall i | 0<i<|c|-1
-        {
-            in_out_circuit_local_lemma(g, c, i);
-        }
-    }
+    // lemma in_out_circuit_lemma(g: Graph, c: seq<nat>)
+    //     requires validUndirectedGraph(g)
+    //     requires |g|>2 && |g|%3==0
+    //     requires isUndirectedHamiltonianCircuit(g, c)
+    //     requires in_out_graph(g)
+    //     ensures in_out_circuit(g, c)
+    // {
+    //     assert (forall i :: 0<i<|c|-1 ==> way2(g, c, i)) ==> (forall i :: 0<i<|c|-1 ==> way1(g, rSeq(c), i));
+    //     forall i | 0<i<|c|-1
+    //     {
+    //         in_out_circuit_local_lemma(g, c, i);
+    //     }
+    // }
 
-    lemma in_out_circuit_local_lemma(g: Graph, c: seq<nat>, i: int)
-        requires validUndirectedGraph(g)
-        requires |g|>2 && |g|%3==0
-        requires isUndirectedHamiltonianCircuit(g, c)
-        requires in_out_graph(g)
-        requires 0<i<|c|-1
-        ensures way1(g, c, i)
-    {
-        if 0<=c[i]<|g|/3
-        {
-            in_out_circuit_1_lemma(g, c, i);
-            // assume c[i-1]==c[i]+(|g|/3)*2 && c[i+1]==c[i]+|g|/3;
-        }
-        if |g|/3<=c[i]<(|g|/3)*2
-        {
-            in_out_circuit_2_lemma(g, c, i);
-            // assume c[i-1]==c[i]-|g|/3 && (|g|/3)*2<=c[i+1]<|g|;
-        }
-        if (|g|/3)*2<=c[i]<|g|
-        {
-            in_out_circuit_3_lemma(g, c, i);
-            // assume |g|/3<=c[i-1]<(|g|/3)*2 && c[i+1]==c[i]-(|g|/3)*2;
-        }
-    }
+    // lemma in_out_circuit_local_lemma(g: Graph, c: seq<nat>, i: int)
+    //     requires validUndirectedGraph(g)
+    //     requires |g|>2 && |g|%3==0
+    //     requires isUndirectedHamiltonianCircuit(g, c)
+    //     requires in_out_graph(g)
+    //     requires 0<i<|c|-1
+    //     ensures way1(g, c, i)
+    // {
+    //     if 0<=c[i]<|g|/3
+    //     {
+    //         in_out_circuit_1_lemma(g, c, i);
+    //         // assume c[i-1]==c[i]+(|g|/3)*2 && c[i+1]==c[i]+|g|/3;
+    //     }
+    //     if |g|/3<=c[i]<(|g|/3)*2
+    //     {
+    //         in_out_circuit_2_lemma(g, c, i);
+    //         // assume c[i-1]==c[i]-|g|/3 && (|g|/3)*2<=c[i+1]<|g|;
+    //     }
+    //     if (|g|/3)*2<=c[i]<|g|
+    //     {
+    //         in_out_circuit_3_lemma(g, c, i);
+    //         // assume |g|/3<=c[i-1]<(|g|/3)*2 && c[i+1]==c[i]-(|g|/3)*2;
+    //     }
+    // }
 
 
-    lemma in_out_circuit_1_lemma(g: Graph, c: seq<nat>, i: int)
-        requires validUndirectedGraph(g)
-        requires |g|>2 && |g|%3==0
-        requires isUndirectedHamiltonianCircuit(g, c)
-        requires in_out_graph(g)
-        requires 0<i<|c|-1
-        requires 0<=c[i]<|g|/3
-        ensures c[i-1]==c[i]+(|g|/3)*2 || c[i+1]==c[i]+(|g|/3)*2
-    {}
+    // lemma in_out_circuit_1_lemma(g: Graph, c: seq<nat>, i: int)
+    //     requires validUndirectedGraph(g)
+    //     requires |g|>2 && |g|%3==0
+    //     requires isUndirectedHamiltonianCircuit(g, c)
+    //     requires in_out_graph(g)
+    //     requires 0<i<|c|-1
+    //     requires 0<=c[i]<|g|/3
+    //     ensures c[i-1]==c[i]+(|g|/3)*2 || c[i+1]==c[i]+(|g|/3)*2
+    // {}
     
-    lemma in_out_circuit_2_lemma(g: Graph, c: seq<nat>, i: int)
-        requires validUndirectedGraph(g)
-        requires |g|>2 && |g|%3==0
-        requires isUndirectedHamiltonianCircuit(g, c)
-        requires in_out_graph(g)
-        requires 0<i<|c|-1
-        requires |g|/3<=c[i]<(|g|/3)*2
-        ensures c[i-1]==c[i]-|g|/3 && (|g|/3)*2<=c[i+1]<|g|
-    {}
+    // lemma in_out_circuit_2_lemma(g: Graph, c: seq<nat>, i: int)
+    //     requires validUndirectedGraph(g)
+    //     requires |g|>2 && |g|%3==0
+    //     requires isUndirectedHamiltonianCircuit(g, c)
+    //     requires in_out_graph(g)
+    //     requires 0<i<|c|-1
+    //     requires |g|/3<=c[i]<(|g|/3)*2
+    //     ensures c[i-1]==c[i]-|g|/3 && (|g|/3)*2<=c[i+1]<|g|
+    // {}
 
-    lemma in_out_circuit_3_lemma(g: Graph, c: seq<nat>, i: int)
-        requires validUndirectedGraph(g)
-        requires |g|>2 && |g|%3==0
-        requires isUndirectedHamiltonianCircuit(g, c)
-        requires in_out_graph(g)
-        requires 0<i<|c|-1
-        requires (|g|/3)*2<=c[i]<|g|
-        ensures |g|/3<=c[i-1]<(|g|/3)*2 && c[i+1]==c[i]-(|g|/3)*2 
-    {}
+    // lemma in_out_circuit_3_lemma(g: Graph, c: seq<nat>, i: int)
+    //     requires validUndirectedGraph(g)
+    //     requires |g|>2 && |g|%3==0
+    //     requires isUndirectedHamiltonianCircuit(g, c)
+    //     requires in_out_graph(g)
+    //     requires 0<i<|c|-1
+    //     requires (|g|/3)*2<=c[i]<|g|
+    //     ensures |g|/3<=c[i-1]<(|g|/3)*2 && c[i+1]==c[i]-(|g|/3)*2 
+    // {}
 
     // ghost function in_out_to_directed(g: Graph): Graph
     //     requires validUndirectedGraph(g)
@@ -238,5 +238,167 @@ module LeftLemma
     //     else if 0<=uc[0]<|g|/3 then cicle_sequence(uc, 1)   //0: og -> put [0,1] at the end
     //     else uc //0: in -> already std
     // }
+
+    // lemma lem(g: Graph, g': Graph)
+    //     requires validGraph(g)
+    //     requires |g|>0
+    //     requires g' == directed_to_undirected_graph(g)
+    //     requires directedHamiltonianCircuit(reverse_rFunction(g'))
+    //     ensures directedHamiltonianCircuit(g)
+    // {}
+
+    lemma lem(g: Graph, c: seq<nat>)
+        requires validUndirectedGraph(g)
+        requires |g|>2 && |g|%3==0
+        requires in_out_graph(g)
+        requires undirectedHamiltonianCircuit(g)
+        ensures directedHamiltonianCircuit(reverse_rFunction(g))
+    {
+        var g' := reverse_rFunction(g);
+
+        assert |g'|>0;
+        var uhc :| isUndirectedHamiltonianCircuit(g, uhc);
+
+        var dhc_eq := circuit_reverse_equivalence(g, g', uhc);
+        
+    }
+
+    ghost function reverse_rFunction(g: Graph): Graph
+        requires validUndirectedGraph(g)
+        requires |g|>2 && |g|%3==0
+        requires in_out_graph(g)
+        //remove in and out nodes
+        ensures |reverse_rFunction(g)| == |g|/3
+        //squared matrix
+        ensures validGraph(reverse_rFunction(g))
+        //direction relation: n1->n2 only and only if n1_out->n2_in
+        ensures forall f :: 0<=f<|g|/3 ==> (forall c :: 0<=c<|g|/3 ==> (g[f+|g|/3][c+(|g|/3)*2] <==> reverse_rFunction(g)[f][c]))
+    {
+        var g_aux := collapsed_graph(g);
+        reverse_rFunction_(g, g_aux, |g_aux|-1)
+    }
+
+    ghost function collapsed_graph(g: Graph): Graph
+        requires validUndirectedGraph(g)
+        requires |g|>2 && |g|%3==0
+        ensures validGraph(collapsed_graph(g))
+        ensures |collapsed_graph(g)|==|g|/3
+        ensures unconnected_graph(collapsed_graph(g))
+    {
+        seq(|g|/3, i => seq(|g|/3, i => false))
+    }
+
+    ghost function reverse_rFunction_(g: Graph, g': Graph, i: int): Graph
+        requires validUndirectedGraph(g)
+        requires |g|>2 && |g|%3==0
+        requires validGraph(g')
+        requires |g'|==|g|/3
+        requires unconnected_graph(g')
+        requires -1<=i<|g'|
+        ensures validGraph(reverse_rFunction_(g, g', i))
+        ensures |reverse_rFunction_(g, g', i)| == |g'|
+        //every row yet to process stay the same
+        ensures forall f :: i< f<|g'| ==> (g'[f] == reverse_rFunction_(g, g', i)[f])
+        //modifying property: for every processed row: n to c in g' if and only if n_out to c_in in g
+        ensures forall f :: 0<=f<=i ==>
+        (
+            forall c :: 0<=c<|g'| ==> (g[f+|g|/3][c+(|g|/3)*2] <==> reverse_rFunction_(g, g', i)[f][c])
+        )
+    {
+        if i==-1 then g' else
+            var g'' := reverse_rFunction_(g, g', i-1);
+            process_out_node_connections(g, g'', i, |g'|-1)
+    }
+
+    //for n and for every other node i: if n_out->i_in ==> n->i
+    ghost function process_out_node_connections(g: Graph, g': Graph, n: int, i: int): Graph
+        requires validUndirectedGraph(g)
+        requires |g|>2 && |g|%3==0
+        requires validGraph(g')
+        requires |g'|==|g|/3
+        requires 0<=n<|g'|
+        requires -1<=i<|g'|
+        //row set to false
+        requires forall c :: 0<=c<|g'| ==> !g'[n][c]
+        ensures validGraph(process_out_node_connections(g, g', n, i))
+        ensures |process_out_node_connections(g, g', n, i)| == |g'|
+        //only n's row is modified
+        ensures forall f :: 0<=f<|g'| && f!=n ==> (g'[f] == process_out_node_connections(g, g', n, i)[f])
+        //only n->x vertex are modified,
+        // ensures forall c :: 0<=c<|g'| ==> (g'[n][c] == direction_equivalence_node_(g, g', n, i)[n][c])
+        //inductive postconditions:
+        //every column yet to process stays the same (set to false)
+        ensures forall c :: i< c<|g'| ==> (g'[n][c] == process_out_node_connections(g, g', n, i)[n][c])
+        //modifying property: n to i in g' if and only if n_out to i_in in g
+        ensures forall c :: 0<=c<=i ==>
+        (
+            g[n+|g|/3][c+(|g|/3)*2] <==> process_out_node_connections(g, g', n, i)[n][c]
+        )
+    {
+        if i==-1 then g' else
+            var g'' := process_out_node_connections(g, g', n, i-1);
+            if g[n+|g|/3][i+(|g|/3)*2] then
+                var f_aux1 := g''[n];
+                var f_aux2 := f_aux1[..i]+[true]+f_aux1[i+1..];
+                var gF := g''[n := f_aux2];
+                gF
+            else
+                g''
+    }
+
+
+    ghost function circuit_reverse_equivalence(g: Graph, g': Graph, circuit: seq<nat>): seq<nat>
+        requires validUndirectedGraph(g)
+        requires |g|>2 && |g|%3==0
+        requires in_out_graph(g)
+        requires isUndirectedHamiltonianCircuit(g, circuit)
+        requires g' == reverse_rFunction(g)
+        ensures isDirectedHamiltonianCircuit(g', circuit_reverse_equivalence(g, g', circuit))
+    {
+        circuit_reverse_equivalence_(g, g', circuit, |g'|-1)
+    }
+
+    ghost function circuit_reverse_equivalence_(g: Graph, g': Graph, c: seq<nat>, i: int): seq<nat>
+        requires validUndirectedGraph(g)
+        requires |g|>2 && |g|%3==0
+        requires in_out_graph(g)
+        requires isUndirectedHamiltonianCircuit(g, c)
+        requires g' == reverse_rFunction(g)
+        requires -1<=i<|c|
+        decreases i
+        ensures |circuit_reverse_equivalence_(g, g', c, i)| == (i+1)/3
+    {
+        if i==-1 then [] else
+            var c' := circuit_reverse_equivalence_(g, g', c, i-1);
+            if 0<c[i]<|g'| then c'+[c[i]] else c'
+    }
+
+    lemma in_out_circuit_property_lemma(g: Graph, c: seq<nat>)
+        requires validUndirectedGraph(g)
+        requires |g|>2 && |g|%3==0
+        requires in_out_graph(g)
+        requires isUndirectedHamiltonianCircuit(g, c)
+        requires (|g|/3)*2<=c[0]<|g| && 0<=c[1]<|g|/3
+    {
+        assert |c|%3==0;
+        var triplets := partition_into_triplets(c);
+        assert forall t :: t in triplets ==> ((|g|/3)*2<=t[0]<|g| && 0<=t[1]<|g|/3 && |g|/3<=t[2]<(|g|/3*2));
+    }
+
+    ghost function partition_into_triplets(s: seq<nat>): seq<seq<nat>>
+        requires |s|%3==0
+        ensures |partition_into_triplets(s)| == |s| / 3
+        ensures forall i :: 0 <= i < |partition_into_triplets(s)| ==> |partition_into_triplets(s)[i]| == 3
+        ensures s == boom(partition_into_triplets(s))
+    {
+        if |s| == 0 then [] else
+            [s[0..3]] + partition_into_triplets(s[3..])
+    }
+
+    function boom(seqs: seq<seq<nat>>): seq<nat>
+        decreases seqs
+    {
+        if |seqs| == 0 then [] else seqs[0] + boom(seqs[1..])
+    }
 
 }
